use bspec contract in mod2, leaves 2 cheats

examples/riscv/mod2/mod2_specScript.sml
@@ -2,6 +2,8 @@ open HolKernel boolLib Parse bossLib;
 
 open markerTheory;
 
+open wordsTheory;
+
 open distribute_generic_stuffLib;
 
 open bir_programSyntax bir_program_labelsTheory;
@@ -17,6 +19,7 @@ open bir_typing_expTheory;
 open bir_htTheory;
 
 open tutorial_smtSupportLib;
+open birs_smtLib;
 
 open bir_symbTheory birs_auxTheory;
 open HolBACoreSimps;
@@ -41,58 +44,52 @@ open program_logicSimps;
 open bir_env_oldTheory;
 open bir_program_varsTheory;
 
-open mod2Theory;
-
 open distribute_generic_stuffTheory;
+
+open mod2Theory;
 
 val _ = new_theory "mod2_spec";
 
-(* --------------- *)
-(* HLSPEC          *)
 (* --------------- *)
 (* RISC-V contract *)
 (* --------------- *)
 
 Definition riscv_mod2_pre_def:
- riscv_mod2_pre x (m : riscv_state) =
-  (m.c_gpr m.procID 10w = n2w x)
+ riscv_mod2_pre (x:word64) (m : riscv_state) =
+  (m.c_gpr m.procID 10w = x)
 End
 
 Definition riscv_mod2_post_def:
- riscv_mod2_post x (m : riscv_state) =
-  (m.c_gpr m.procID 10w = n2w (x MOD 2))
+ riscv_mod2_post (x:word64) (m : riscv_state) =
+  (m.c_gpr m.procID 10w = n2w ((w2n x) MOD 2))
 End
 
-(* ------------ *)
-(* HLSPEC       *)
-(* ------------ *)
-(* BIR contract *)
-(* ------------ *)
+(* --------------- *)
+(* HL BIR contract *)
+(* --------------- *)
 
 Definition bir_mod2_pre_def:
-  bir_mod2_pre x : bir_exp_t =
+ bir_mod2_pre (x:word64) : bir_exp_t =
   BExp_BinPred
     BIExp_Equal
     (BExp_Den (BVar "x10" (BType_Imm Bit64)))
-    (BExp_Const (Imm64 (n2w x)))
+    (BExp_Const (Imm64 x))
 End
 
 Definition bir_mod2_post_def:
- bir_mod2_post x : bir_exp_t =
+ bir_mod2_post (x:word64) : bir_exp_t =
   BExp_BinPred
     BIExp_Equal
     (BExp_Den (BVar "x10" (BType_Imm Bit64)))
-    (BExp_Const (Imm64 (n2w (x MOD 2))))
+    (BExp_Const (Imm64 (n2w ((w2n x) MOD 2))))
 End
 
-(* ------------ *)
-(* BSPEC        *)
-(* ------------ *)
-(* BIR contract *)
-(* ------------ *)
+(* -------------- *)
+(* BSPEC contract *)
+(* -------------- *)
 
 Definition bspec_mod2_pre_def:
-  bspec_mod2_pre x : bir_exp_t =
+ bspec_mod2_pre (x:word64) : bir_exp_t =
   BExp_BinPred
    BIExp_Equal
    (BExp_Den (BVar "x10" (BType_Imm Bit64)))
@@ -100,7 +97,7 @@ Definition bspec_mod2_pre_def:
 End
 
 Definition bspec_mod2_post_def:
- bspec_mod2_post x : bir_exp_t =
+ bspec_mod2_post (x:word64) : bir_exp_t =
   BExp_BinPred
     BIExp_Equal
     (BExp_Den (BVar "x10" (BType_Imm Bit64)))
@@ -108,9 +105,9 @@ Definition bspec_mod2_post_def:
       BIExp_And (BExp_Const (Imm64 x)) (BExp_Const (Imm64 1w)))
 End
 
-(* ----------------------------------- *)
-(* Connecting RISC-V and BIR contracts *)
-(* ----------------------------------- *)
+(* -------------------------------------- *)
+(* Connecting RISC-V and HL BIR contracts *)
+(* -------------------------------------- *)
 
 Theorem mod2_riscv_pre_imp_bir_pre_thm:
  bir_pre_riscv_to_bir (riscv_mod2_pre pre_x10) (bir_mod2_pre pre_x10)
@@ -134,48 +131,57 @@ Proof
   (FULL_SIMP_TAC (std_ss++holBACore_ss) [bir_eval_bin_pred_def] >>
    fs [Abbrev_def] >>
    `bir_eval_bin_pred BIExp_Equal (SOME z)
-     (SOME (BVal_Imm (Imm64 (n2w (pre_x10 MOD 2))))) = SOME bir_val_true`
+     (SOME (BVal_Imm (Imm64 (n2w ((w2n pre_x10) MOD 2))))) = SOME bir_val_true`
     by METIS_TAC [] >>
    Cases_on `z` >> fs [type_of_bir_val_def] >>
    FULL_SIMP_TAC (std_ss++holBACore_ss) [bir_eval_bin_pred_def,bir_immTheory.bool2b_def,bir_val_true_def] >>
    FULL_SIMP_TAC (std_ss++holBACore_ss) [bool2w_def] >>
-   Q.ABBREV_TAC `bb = bir_bin_pred BIExp_Equal b' (Imm64 (n2w (pre_x10 MOD 2)))` >>
+   Q.ABBREV_TAC `bb = bir_bin_pred BIExp_Equal b' (Imm64 (n2w ((w2n pre_x10) MOD 2)))` >>
    Cases_on `bb` >> fs [] >>
    FULL_SIMP_TAC (std_ss++holBACore_ss) [bir_exp_immTheory.bir_bin_pred_Equal_REWR] >>
    FULL_SIMP_TAC (std_ss++holBACore_ss) [riscv_bmr_rel_EVAL,bir_envTheory.bir_env_read_def, bir_envTheory.bir_env_check_type_def, bir_envTheory.bir_env_lookup_type_def, bir_envTheory.bir_env_lookup_def,bir_eval_bin_pred_def]) >>
  FULL_SIMP_TAC (std_ss++holBACore_ss) []
 QED
 
-(* ----------------------------------------- *)
-(* Connecting HLSPEC BIR and BSPEC contracts *)
-(* ----------------------------------------- *)
+(* ------------------------------------- *)
+(* Connecting HL BIR and BSPEC contracts *)
+(* ------------------------------------- *)
 
 val mod2_bir_pre_imp_bspec_pre_thm =
  prove_exp_is_taut ``BExp_BinExp BIExp_Or
-   (BExp_UnaryExp BIExp_Not (bir_mod2_pre (w2n pre_x10)))
+   (BExp_UnaryExp BIExp_Not (bir_mod2_pre pre_x10))
    (bspec_mod2_pre pre_x10)``;
 
 Theorem mod2_bir_pre_imp_bspec_pre:
  bir_exp_is_taut (BExp_BinExp BIExp_Or
-   (BExp_UnaryExp BIExp_Not (bir_mod2_pre (w2n pre_x10)))
+   (BExp_UnaryExp BIExp_Not (bir_mod2_pre pre_x10))
    (bspec_mod2_pre pre_x10))
 Proof
  rw [mod2_bir_pre_imp_bspec_pre_thm]
 QED
 
-(*
-val mod2_bspec_post_imp_bir_post_thm =
- prove_exp_is_taut ``BExp_BinExp BIExp_Or
-   (BExp_UnaryExp BIExp_Not (bspec_mod2_post pre_x10))
-    (bir_mod2_post (w2n pre_x10))``;
+Theorem mod2_wand_n2w_w2n[local]:
+ !x. 1w && x = n2w ((w2n x) MOD 2)
+Proof
+ STRIP_TAC >>
+ MP_TAC (Q.SPECL [`1`, `w2n x`] WORD_AND_EXP_SUB1) >>
+ rw []
+QED
+
+Theorem mod2_wand_1w_bval_imm[local]:
+ !x v.
+  BVal_Imm (Imm64 (1w && x)) = v ==>
+  v = BVal_Imm (Imm64 (n2w ((w2n x) MOD 2)))
+Proof
+ fs [] >> rw [mod2_wand_n2w_w2n]
+QED
 
 Theorem mod2_bspec_post_imp_bir_post:
  bir_exp_is_taut (BExp_BinExp BIExp_Or
    (BExp_UnaryExp BIExp_Not (bspec_mod2_post pre_x10))
     (bir_mod2_post pre_x10))
 Proof
- rw [mod2_bspec_post_imp_bir_post_thm]
+ cheat
 QED
-*)
 
 val _ = export_theory ();
